\section{Introduction to the $\Gamma$ Function}
\begin{define}[$\Gamma$ function]
  \index{gamma function}
  \[
    \Gamma(z) = \int_{0}^{\infty} x^{z-1} e^{-x} \mathrm{d}x
  \]
  \tcblower
  Though $x^z$ may seems more natural, wiki just defines it like this.
\end{define}
$\Gamma$ function is a very useful function, it could represent the factorial not in whole nummber but also in real number.
\begin{proposition}[]
  \[
    \Gamma(z+1) = z\Gamma(z)
  \]
\end{proposition}
\begin{proof}
  \begin{align*}
    (-x^ze^{-x})' &= x^ze^{-x} + (-zx^{z-1}e^{-x})\\
    \left[-x^ze^{-x}\right]_0^\infty &= \int_0^\infty x^ze^{-x} \mathrm{d}x + \int_0^\infty -zx^{z-1}e^{-x}\mathrm{d}x \\
    \int_0^\infty x^ze^{-x}\mathrm{d}x &= \left[-x^ze^{-x}\right]_0^\infty + \int_0^\infty zx^{z-1}e^{-x}\mathrm{d}x \\
    \int_0^\infty x^ze^{-x}\mathrm{d}x &=  z\int_0^\infty x^{z-1}e^{-x}\mathrm{d}x \\
    \Gamma(z+1) &= z\Gamma(z) \qedhere
  \end{align*}
  \textbf{Actually, all the $\infty$ here means $+\infty$.}
\end{proof}
\begin{proposition}[]
  \[
    \Gamma(1) = 1
  \]
\end{proposition}
\begin{proof}
  \begin{align*}
    \Gamma(1) &= \int_0^\infty x^{1-1}e^{-x} \mathrm{d}x \\
              &= \int_0^\infty e^{-x} \mathrm{d}x \\
              &= \left[-e^{-x}\right]_0^\infty \\
              &= \lim_{x\to \infty}-e^{-x} + e^0 \\
              &= 0 + 1 \\
              &= 1 \qedhere
  \end{align*}
  \textbf{Actually, all the $\infty$ here means $+\infty$.}
\end{proof}
\begin{corollary}[]
  \[\Gamma(z) = (z-1)!\]
\end{corollary}
%%% Local Variables:
%%% mode: latex
%%% TeX-master: "../../notebook"
%%% End:
